AESGCM.v
@@ -1,0 +1,117 @@
+Set Implicit Arguments.
+
+Require Import AES.
+Require Import GCM.
+Require Import EncryptionInterface.
+
+Module AESGCM <: EncryptionAlgorithm EncryptionStringDataTypes.
+
+  Import EncryptionStringDataTypes.
+
+  Require Import FPUtil.
+  Require Import Arith NArith NPeano Ascii String List Bool.
+  Import ListNotations.
+  Local Open Scope prog_scope.
+  Local Open Scope N_scope.
+  Local Open Scope nat_scope.
+  Local Open Scope string_scope.
+  Local Open Scope list_scope.
+  Local Open Scope bool_scope.
+  Require Import Bitvec.
+  Local Open Scope bitvec_scope.
+
+  Local Notation bits := str_to_bitvec.
+  Local Notation "# s" := (bits s) (at level 0).
+  Local Notation str := bitvec_to_str.
+
+  Infix "=?" := beq_nat : nat_scope.
+  Infix "<>?" := bne_nat (at level 70) : nat_scope.
+
+  Definition isValidMasterKey (key : masterKeyT) : bool := (length #key =? 128)%nat.
+
+  Definition randomnessHint (rawData : rawDataT) : systemRandomnessHintT := 96.
+
+  Definition encrypt (randomness : systemRandomnessT)
+             (masterKey : masterKeyT)
+             (masterKeyValid : isValidMasterKey masterKey = true)
+             (rawData : rawDataT):
+    encryptedDataT + EncryptionError systemRandomnessHintT systemRandomnessT :=
+    let IV := #randomness in
+    let IV_len := length IV in
+    if  IV_len <? 96 then inr $ NotEnoughRandomness _ _ 96 randomness
+    else
+      let IV := firstn 96 IV in
+      let (C, T) := GCM.encrypt AES.encrypt #masterKey IV #rawData [] 128 in
+      inl $ str $ IV ++ T ++ C.
+
+  Definition decrypt (masterKey : masterKeyT)
+             (masterKeyValid : isValidMasterKey masterKey = true)
+             (encryptedData : encryptedDataT) :
+    rawDataT + DecryptionError :=
+    let err := inr $ InvalidEncryptedData in
+    let C := #encryptedData in
+    if length C <? 96 + 128 then err
+    else
+      let (IV, C) := splitn 96 C in
+      let (T, C) := splitn 128 C in
+      match GCM.decrypt AES.encrypt #masterKey IV C [] T with
+        | Some P => inl $ str $ P
+        | None => err
+      end.
+
+  Lemma is_retraction : forall randomness masterKey masterKeyValid rawData,
+                          let enc := encrypt randomness masterKey masterKeyValid rawData in
+                          match enc with
+                            | inl enc' => decrypt masterKey masterKeyValid enc' = inl rawData
+                            | inr _ => True
+                          end.
+  Proof.
+    admit.
+  Qed.
+
+  Definition doit (x : encryptedDataT + EncryptionError systemRandomnessHintT systemRandomnessT) :=
+    match x with
+      | inl s => s
+      | _ => ""
+    end.
+
+  Definition check (x : rawDataT + DecryptionError) :=
+    match x with
+      | inl s => Some s
+      | _ => None
+    end.
+  
+  Arguments tl {A} _.
+  Arguments removelast {A} _.
+
+  Module test1.
+    Definition K := "2kllajsf3jrl;kaj".
+    Definition R := "9u8jg3q84-u8".
+    Definition P := "8aIOw;fj8dfu[jqoir2wf[usjaiovu9r[2iojd0fawfs293jfE".
+    Definition C := doit $ encrypt R K eq_refl P.
+    Goal (check $ decrypt K eq_refl $ C) = Some P. r. Qed.
+    Definition bad1 := list_to_str $ tl $ str_to_list $ C.
+    Goal (check $ decrypt K eq_refl $ bad1) = None. r. Qed.
+    Definition bad2 := list_to_str $ removelast $ str_to_list $ C.
+    Goal (check $ decrypt K eq_refl $ bad2) = None. r. Qed.
+    Definition replace3 := str_to_list "lajsfakls".
+    Definition bad3 :=  list_to_str $ replace3 ++ skipn (length replace3) (str_to_list C).
+    Goal (check $ decrypt K eq_refl $ bad3) = None. r. Qed.
+  End test1.
+
+  Module test2.
+    Definition K := "9ap8usdjfaspd98f".
+    Definition R := "as;jfafsioj;".
+    Definition P := "".
+    Definition C := doit $ encrypt R K eq_refl P.
+    Goal (check $ decrypt K eq_refl $ C) = Some P. r. Qed.
+    Definition bad1 := list_to_str $ tl $ str_to_list $ C.
+    Goal (check $ decrypt K eq_refl $ bad1) = None. r. Qed.
+    Definition bad2 := list_to_str $ removelast $ str_to_list $ C.
+    Goal (check $ decrypt K eq_refl $ bad2) = None. r. Qed.
+    Definition replace3 := str_to_list "lajsfakls".
+    Definition bad3 :=  list_to_str $ replace3 ++ skipn (length replace3) (str_to_list C).
+    Goal (check $ decrypt K eq_refl $ bad3) = None. r. Qed.
+  End test2.
+
+End AESGCM.
